Generalize phis
After    | File Name                            | Before   || Change
-----------------------------------------------------------------------
3m56.20s | Total                                | 4m14.86s || -0m18.66s
-----------------------------------------------------------------------
0m02.44s | Specific/X25519/C32/ReificationTypes | 0m19.48s || -0m17.03s
2m00.12s | Specific/X25519/C64/ladderstep       | 1m55.72s || +0m04.40s
0m01.16s | Specific/X25519/C64/ReificationTypes | 0m05.17s || -0m04.00s
0m26.27s | Specific/X25519/C32/fesquare         | 0m27.76s || -0m01.49s
0m52.60s | Specific/X25519/C32/femul            | 0m52.46s || +0m00.14s
0m10.35s | Specific/X25519/C64/femul            | 0m10.28s || +0m00.07s
0m08.30s | Specific/IntegrationTestSub          | 0m08.69s || -0m00.38s
0m07.97s | Specific/IntegrationTestFreeze       | 0m08.00s || -0m00.03s
0m06.99s | Specific/X25519/C64/fesquare         | 0m07.31s || -0m00.31s

src/Specific/X25519/C32/femul.v
@@ -6,13 +6,10 @@ Require Import Crypto.Util.BoundedWord.
 Require Import Crypto.Specific.IntegrationTestTemporaryMiscCommon.
 Require Import Crypto.Compilers.Z.Bounds.Pipeline.
 
-Local Definition phi : feBW -> F m :=
-  fun x => B.Positional.Fdecode wt (BoundedWordToZ _ _ _ x).
-
 (* TODO : change this to field once field isomorphism happens *)
 Definition mul :
   { mul : feBW -> feBW -> feBW
-  | forall a b, phi (mul a b) = F.mul (phi a) (phi b) }.
+  | forall a b, phiBW (mul a b) = F.mul (phiBW a) (phiBW b) }.
 Proof.
   start_preglue.
   do_rewrite_with_2sig_add_carry mul_sig carry_sig; cbv_runtime.
