src/Specific/X25519/C32/ReificationTypes.v
@@ -1,8 +1,10 @@
 Require Import Coq.ZArith.ZArith.
+Require Import Coq.romega.ROmega.
 Require Import Coq.Lists.List.
 Local Open Scope Z_scope.
 
 Require Import Crypto.Arithmetic.Core.
+Require Import Crypto.Arithmetic.PrimeFieldTheorems.
 Require Import Crypto.Util.FixedWordSizes.
 Require Import Crypto.Util.Tuple.
 Require Import Crypto.Util.ZRange Crypto.Util.BoundedWord.
@@ -13,17 +15,16 @@ Section BoundedField.
   Local Coercion Z.of_nat : nat >-> Z.
 
   Let limb_widths := Eval vm_compute in (List.map (fun i => Z.log2 (wt (S i) / wt i)) (seq 0 sz)).
-  Let length_lw := Eval compute in List.length limb_widths.
 
   Local Notation b_of exp := {| lower := 0 ; upper := P.upper_bound_of_exponent exp |}%Z (only parsing). (* max is [(0, 2^(exp+2) + 2^exp + 2^(exp-1) + 2^(exp-3) + 2^(exp-4) + 2^(exp-5) + 2^(exp-6) + 2^(exp-10) + 2^(exp-12) + 2^(exp-13) + 2^(exp-14) + 2^(exp-15) + 2^(exp-17) + 2^(exp-23) + 2^(exp-24))%Z] *)
   (* The definition [bounds_exp] is a tuple-version of the
      limb-widths, which are the [exp] argument in [b_of] above, i.e.,
      the approximate base-2 exponent of the bounds on the limb in that
      position. *)
-  Let bounds_exp : Tuple.tuple Z length_lw
+  Let bounds_exp : Tuple.tuple Z sz
     := Eval compute in
-        Tuple.from_list length_lw limb_widths eq_refl.
-  Let bounds : Tuple.tuple zrange length_lw
+        Tuple.from_list sz limb_widths eq_refl.
+  Let bounds : Tuple.tuple zrange sz
     := Eval compute in
         Tuple.map (fun e => b_of e) bounds_exp.
 
@@ -39,13 +40,19 @@ Section BoundedField.
     : 0 <= B.Positional.eval wt (BoundedWordToZ sz bitwidth bounds a) < 2 * Z.pos m.
   Proof.
     destruct a as [a H]; unfold BoundedWordToZ, proj1_sig.
-    revert H.
-    cbv -[Z.le Z.add Z.mul Z.lt fst snd wordToZ wt]; cbn [fst snd].
+    destruct_head_hnf' and.
+    cbv -[Z.le Z.add Z.mul Z.lt fst snd wordToZ wt] in *; cbn [fst snd] in *.
     repeat match goal with
+           | [ |- context[@wordToZ ?n ?x] ]
+             => generalize dependent (@wordToZ n x); intros
            | [ |- context[wt ?n] ]
              => let v := (eval compute in (wt n)) in change (wt n) with v
            end.
-    intro; destruct_head'_and.
-    omega.
+    romega.
   Qed.
+
+  Definition phiW : feW -> F m :=
+    fun x => B.Positional.Fdecode wt (Tuple.map wordToZ x).
+  Definition phiBW : feBW -> F m :=
+    fun x => B.Positional.Fdecode wt (BoundedWordToZ _ _ _ x).
 End BoundedField.
