src/Specific/X25519/C64/fesquare.v
@@ -6,13 +6,10 @@ Require Import Crypto.Util.BoundedWord.
 Require Import Crypto.Specific.IntegrationTestTemporaryMiscCommon.
 Require Import Crypto.Compilers.Z.Bounds.Pipeline.
 
-Local Definition phi : feBW -> F m :=
-  fun x => B.Positional.Fdecode wt (BoundedWordToZ _ _ _ x).
-
 (* TODO : change this to field once field isomorphism happens *)
 Definition square :
   { square : feBW -> feBW
-  | forall a, phi (square a) = F.mul (phi a) (phi a) }.
+  | forall a, phiBW (square a) = F.mul (phiBW a) (phiBW a) }.
 Proof.
   start_preglue.
   do_rewrite_with_1sig_add_carry square_sig carry_sig; cbv_runtime.
